Structural Refactoring

LambdaCalculus/Diamond.dfy
@@ -1,5 +1,7 @@
-include "Confluence.dfy"
 include "BetaReduction.dfy"
+include "LemmaA5AndA6.dfy"
+include "LemmaA4.dfy"
+include "LemmaA3.dfy"
 
 lemma {:vcs_split_on_every_assert}DiamondLemma (M:LambdaTerm,M1:LambdaTerm,M2:LambdaTerm)
     requires parallelReduction(M,M1)
@@ -313,95 +315,3 @@ lemma {:vcs_split_on_every_assert}DiamondLemma (M:LambdaTerm,M1:LambdaTerm,M2:La
     }
 }
 
-ghost predicate parallelReductionInNSteps(t1:LambdaTerm,t2:LambdaTerm,n:nat)
-    decreases n
-{
-    if n==0 then alphaEquivalence(t1,t2)
-    else 
-    exists t':LambdaTerm:: parallelReduction(t1,t') && parallelReductionInNSteps(t',t2,n-1)
-}
-
-ghost predicate parallelReductionClosure(t1:LambdaTerm,t2:LambdaTerm)
-{
-    exists n:nat::parallelReductionInNSteps(t1,t2,n)
-}
-
-lemma parallelReductionClosureReflexive(t1:LambdaTerm)
-    ensures parallelReductionClosure(t1,t1)
-{
-    EqualTermsAreAlphaEquilvalent(t1,t1);
-    assert alphaEquivalence(t1,t1);
-    assert parallelReductionInNSteps(t1,t1,0);
-}
-lemma ParClosurePrepend(a:LambdaTerm, b:LambdaTerm, c:LambdaTerm)   
-    requires parallelReduction(a, b)
-    requires parallelReductionClosure(b, c)
-    ensures parallelReductionClosure(a, c)
-{
-    var n:nat :| parallelReductionInNSteps(b, c, n);
-    assert parallelReductionInNSteps(a, c, n+1);     
-}
-lemma StripLemma(a:LambdaTerm,b:LambdaTerm,c:LambdaTerm,n:nat)
-    requires parallelReduction(a, b)
-    requires parallelReductionInNSteps(a, c, n)
-    ensures exists d:LambdaTerm ::parallelReductionClosure(b, d) && parallelReduction(c, d)
-    decreases n
-{
-    if n==0{
-        assert alphaEquivalence(a,c);
-        assert parallelReduction(a,b);
-        EqualTermsAreAlphaEquilvalent(b,b);
-        ParallelReductionAlphaInvariance(a,b,c,b);
-        assert parallelReduction(b,b);
-        assert parallelReduction(c,b);
-        assert parallelReductionInNSteps(b,b,0);
-        assert parallelReductionInNSteps(c,b,1);
-
-    }
-    else
-    {
-        var a1 :| parallelReduction(a, a1) && parallelReductionInNSteps(a1, c, n-1);
-        DiamondLemma(a, b, a1);                    
-        var e :| parallelReduction(b, e) && parallelReduction(a1, e);
-        StripLemma(a1, e, c, n-1);                  
-        var d :| parallelReductionClosure(e, d) && parallelReduction(c, d);
-        ParClosurePrepend(b, e, d);                    
-        assert parallelReductionClosure(b, d) && parallelReduction(c, d);
-    }
-}
-
-lemma ClosureDiamond(a:LambdaTerm, b:LambdaTerm, c:LambdaTerm, m:nat)
-    requires parallelReductionInNSteps(a, b, m)
-    requires parallelReductionClosure(a, c)
-    ensures exists d:LambdaTerm :: parallelReductionClosure(b, d) && parallelReductionClosure(c, d)
-    decreases m 
-{
-    if (m==0)
-    {
-        assert alphaEquivalence(a, b);
-        AlphaEquivSymmetric(a, b);                
-        ParClosurePrepend(b, a, c);                
-        parallelReductionClosureReflexive(c);     
-        assert parallelReductionClosure(b, c) && parallelReductionClosure(c, c);
-        
-    }
-    else
-    {
-        var a1 :| parallelReduction(a, a1) && parallelReductionInNSteps(a1, b, m-1);
-        var k:nat :| parallelReductionInNSteps(a, c, k);
-        StripLemma(a, a1, c, k);                    
-        var e :| parallelReductionClosure(a1, e) && parallelReduction(c, e);
-        ClosureDiamond(a1, b, e, m-1);             
-        var d :| parallelReductionClosure(b, d) && parallelReductionClosure(e, d);
-        ParClosurePrepend(c, e, d);                
-        assert parallelReductionClosure(b, d) && parallelReductionClosure(c, d);
-    }
-}
-lemma ParallelClosureHasDiamond(a:LambdaTerm, b:LambdaTerm, c:LambdaTerm)
-    requires parallelReductionClosure(a, b)
-    requires parallelReductionClosure(a, c)
-    ensures exists d:LambdaTerm :: parallelReductionClosure(b, d) && parallelReductionClosure(c, d)
-{
-    var m:nat :| parallelReductionInNSteps(a, b, m);
-    ClosureDiamond(a, b, c, m);
-}
