LambdaCalculus/HelperLemmasForA3.dfy
@@ -1,0 +1,296 @@
+include "LemmaA2.dfy"
+
+lemma ParallelReductionAlphaInvariance(t1: LambdaTerm, t2: LambdaTerm, t1': LambdaTerm, t2': LambdaTerm)
+    requires parallelReduction(t1, t2)
+    requires alphaEquivalence(t1, t1')
+    requires alphaEquivalence(t2, t2')
+    ensures parallelReduction(t1', t2')
+    decreases lHeight(t1), 0
+{
+    if alphaEquivalence(t1, t2) {
+        AlphaEquivSymmetric(t1, t1');
+        AlphaEquivTransitive(t1', t1, t2);
+        AlphaEquivTransitive(t1', t2, t2');
+        return;
+    }
+    match t1 {
+        case Var(z) => {
+            assert false;
+        }
+        case Lambda(x, body1) => {
+            var r :| parallelReduction(body1, r) && alphaEquivalence(Lambda(x, r), t2);
+            NonLambdaAlphaEquivalence(t1, t1');
+            match t1' {
+                case Lambda(x', body1') => {
+                    ParRedAlphaUnderBinder(x, body1, r, x', body1');
+                    var RR :| parallelReduction(body1', RR) && alphaEquivalence(Lambda(x', RR), Lambda(x, r));
+                    AlphaEquivTransitive(Lambda(x', RR), Lambda(x, r), t2);
+                    AlphaEquivTransitive(Lambda(x', RR), t2, t2');
+                    ParRedLambdaIntro(x', body1', RR, t2');
+                }
+                case _ => {}
+            }
+        }
+        case Application(t1a, t1b) => {
+            NonApplicationAlphaEquivalence(t1, t1');
+            match t1' {
+                case Application(t1a', t1b') => {
+                    ApplicationEquivalenceDown(t1a, t1b, t1a', t1b');
+                    if t2.Application? && parallelReduction(t1a, t2.t1) && parallelReduction(t1b, t2.t2) {
+                        NonApplicationAlphaEquivalence(t2, t2');
+                        match t2' {
+                            case Application(t2a', t2b') => {
+                                ApplicationEquivalenceDown(t2.t1, t2.t2, t2a', t2b');
+                                ParallelReductionAlphaInvariance(t1a, t2.t1, t1a', t2a');
+                                ParallelReductionAlphaInvariance(t1b, t2.t2, t1b', t2b');
+                                assert parallelReduction(t1a', t2a') && parallelReduction(t1b', t2b');
+                            }
+                            case _ => {}
+                        }
+                    } else {
+                        match t1a {
+                            case Lambda(x, M) => {
+                                var M', N' :| parallelReduction(M, M') && parallelReduction(t1b, N')
+                                              && alphaEquivalence(t2, caSubstitution(M', x, N'));
+                                NonLambdaAlphaEquivalence(t1a, t1a');
+                                match t1a' {
+                                    case Lambda(x', body') => {
+                                        ParRedAlphaUnderBinder(x, M, M', x', body');
+                                        var M'' :| parallelReduction(body', M'')
+                                                   && alphaEquivalence(Lambda(x', M''), Lambda(x, M'));
+                                        EqualTermsAreAlphaEquilvalent(N', N');
+                                        ParallelReductionAlphaInvariance(t1b, N', t1b', N');
+                                        AlphaEquivSymmetric(Lambda(x', M''), Lambda(x, M'));
+                                        SubstRespectsBinderAlpha(x, M', x', M'', N');
+                                        AlphaEquivSymmetric(t2, t2');
+                                        AlphaEquivTransitive(t2', t2, caSubstitution(M', x, N'));
+                                        AlphaEquivTransitive(t2', caSubstitution(M', x, N'), caSubstitution(M'', x', N'));
+                                        ParRedBetaIntro(x', body', t1b', M'', N', t2');
+                                    }
+                                    case _ => {}
+                                }
+                            }
+                            case _ => {}
+                        }
+                    }
+                }
+                case _ => {}
+            }
+        }
+    }
+}
+lemma {:vcs_split_on_every_assert} ParRedRename(M:LambdaTerm, M':LambdaTerm, a:Id, b:Id)
+    requires parallelReduction(M, M')
+    ensures parallelReduction(caSubstitution(M, a, Var(b)), caSubstitution(M', a, Var(b)))
+    decreases lHeight(M), 1
+{
+    var Mca := caSubstitution(M, a, Var(b));
+    var M'ca := caSubstitution(M', a, Var(b));
+    if alphaEquivalence(M, M') {
+        EqualTermsAreAlphaEquilvalent(Var(b), Var(b));
+        CaSubstEquivalence(M, Var(b), M', Var(b), a);
+        return;
+    }
+    match M {
+        case Var(z) => { assert false; }
+        case Lambda(z, body) => {
+            var s :| parallelReduction(body, s) && alphaEquivalence(Lambda(z, s), M');
+            var S := addition(a, addition(b, reunion(vars(M), reunion(vars(M'), vars(s)))));
+            reunionIncludesBothSets(vars(M'), vars(s));
+            reunionIncludesBothSets(vars(M), reunion(vars(M'), vars(s)));
+            var zf := addAnUniqueId(S)[0];
+            assert !(zf in S);
+            assert zf != a && zf != b;
+            varsOfALambdaIncludesVarsofASubLambda(M);
+            assert !(zf in vars(M)) && !(zf in vars(M')) && !(zf in vars(s));
+            assert !(zf in vars(body));
+
+            var body_alt := substitution(body, z, Var(zf));
+            var s_alt := substitution(s, z, Var(zf));
+
+            ParRedRename(body, s, z, zf);
+            CaSubstIsNaiveWhenFresh(body, z, zf);
+            CaSubstIsNaiveWhenFresh(s, z, zf);
+            assert parallelReduction(body_alt, s_alt);
+
+            subsitutionOfVarDoesNotChangeHeightFORVARIABLES(body, z, Var(zf));
+            ParRedRename(body_alt, s_alt, a, b);
+            var PbA := caSubstitution(body_alt, a, Var(b));
+            var rr := caSubstitution(s_alt, a, Var(b));
+            assert parallelReduction(PbA, rr);
+
+            SubstAlphaEquivalence(body, z, zf);
+            EqualTermsAreAlphaEquilvalent(Var(b), Var(b));
+            CaSubstEquivalence(M, Var(b), Lambda(zf, body_alt), Var(b), a);
+            SubstPushesIntoSafeLambda(zf, body_alt, a, Var(b));
+            AlphaEquivTransitive(Mca, caSubstitution(Lambda(zf, body_alt), a, Var(b)), Lambda(zf, PbA));
+
+            SubstAlphaEquivalence(s, z, zf);
+            AlphaEquivTransitive(Lambda(zf, s_alt), Lambda(z, s), M');
+            CaSubstEquivalence(Lambda(zf, s_alt), Var(b), M', Var(b), a);
+            SubstPushesIntoSafeLambda(zf, s_alt, a, Var(b));
+            AlphaEquivSymmetric(caSubstitution(Lambda(zf, s_alt), a, Var(b)), Lambda(zf, rr));
+            AlphaEquivTransitive(Lambda(zf, rr), caSubstitution(Lambda(zf, s_alt), a, Var(b)), M'ca);
+
+            ParRedLambdaIntro(zf, PbA, rr, M'ca);
+            AlphaEquivSymmetric(Mca, Lambda(zf, PbA));
+            EqualTermsAreAlphaEquilvalent(M'ca, M'ca);
+            CaSubsitutionOfVarDoesNotChangeHeightFORVARIABLES(body_alt, a, Var(b));
+            ParallelReductionAlphaInvariance(Lambda(zf, PbA), M'ca, Mca, M'ca);
+        }
+        case Application(P, Q) => {
+            if M'.Application? && parallelReduction(P, M'.t1) && parallelReduction(Q, M'.t2) {
+                var Pp := M'.t1;
+                var Qp := M'.t2;
+                SubstDistributesOverApp(P, Q, a, Var(b));
+                SubstDistributesOverApp(Pp, Qp, a, Var(b));
+                ParRedRename(P, Pp, a, b);
+                ParRedRename(Q, Qp, a, b);
+                var PA := caSubstitution(P, a, Var(b));
+                var QA := caSubstitution(Q, a, Var(b));
+                var PpA := caSubstitution(Pp, a, Var(b));
+                var QpA := caSubstitution(Qp, a, Var(b));
+                ParRedCongIntro(PA, QA, PpA, QpA);
+                AlphaEquivSymmetric(Mca, Application(PA, QA));
+                AlphaEquivSymmetric(M'ca, Application(PpA, QpA));
+                CaSubsitutionOfVarDoesNotChangeHeightFORVARIABLES(P, a, Var(b));
+                CaSubsitutionOfVarDoesNotChangeHeightFORVARIABLES(Q, a, Var(b));
+                ParallelReductionAlphaInvariance(Application(PA, QA), Application(PpA, QpA), Mca, M'ca);
+            } else {
+                match P {
+                    case Lambda(z, Pb) => {
+                        var Pb', Q'' :| parallelReduction(Pb, Pb') && parallelReduction(Q, Q'')
+                                        && alphaEquivalence(M', caSubstitution(Pb', z, Q''));
+                        var S := addition(a, addition(b, reunion(vars(M), reunion(vars(M'),
+                                    reunion(vars(Pb'), vars(Q''))))));
+                        reunionIncludesBothSets(vars(Pb'), vars(Q''));
+                        reunionIncludesBothSets(vars(M'), reunion(vars(Pb'), vars(Q'')));
+                        reunionIncludesBothSets(vars(M), reunion(vars(M'), reunion(vars(Pb'), vars(Q''))));
+                        var zf := addAnUniqueId(S)[0];
+                        assert !(zf in S);
+                        assert zf != a && zf != b;
+                        varsOfALambdaIncludesVarsofASubLambda(M);
+                        varsOfALambdaIncludesVarsofASubLambda(P);
+                        assert !(zf in vars(M)) && !(zf in vars(M')) && !(zf in vars(Pb')) && !(zf in vars(Q''));
+                        assert !(zf in vars(P));
+                        assert !(zf in vars(Pb)) && !(zf in vars(Q));
+
+                        var Pb_alt := substitution(Pb, z, Var(zf));
+                        var Pb'_alt := substitution(Pb', z, Var(zf));
+
+                        assert parallelReduction(Pb, Pb');
+                        assert lHeight(Pb) < lHeight(M);
+                        ParRedRename(Pb, Pb', z, zf);
+                        CaSubstIsNaiveWhenFresh(Pb, z, zf);
+                        CaSubstIsNaiveWhenFresh(Pb', z, zf);
+                        assert parallelReduction(Pb_alt, Pb'_alt);
+
+                        subsitutionOfVarDoesNotChangeHeightFORVARIABLES(Pb, z, Var(zf));
+                        var PbA := caSubstitution(Pb_alt, a, Var(b));
+                        var QA := caSubstitution(Q, a, Var(b));
+                        var P2 := caSubstitution(Pb'_alt, a, Var(b));
+                        var N2 := caSubstitution(Q'', a, Var(b));
+
+                        ParRedRename(Pb_alt, Pb'_alt, a, b);
+                        ParRedRename(Q, Q'', a, b);
+                        assert parallelReduction(PbA, P2);
+                        assert parallelReduction(QA, N2);
+
+                        var LHSapp := Application(Lambda(zf, PbA), QA);
+
+                        SubstAlphaEquivalence(Pb, z, zf);
+                        EqualTermsAreAlphaEquilvalent(Q, Q);
+                        ApplicationEquivalence(Lambda(z, Pb), Lambda(zf, Pb_alt), Q, Q);
+                        EqualTermsAreAlphaEquilvalent(Var(b), Var(b));
+                        CaSubstEquivalence(M, Var(b), Application(Lambda(zf, Pb_alt), Q), Var(b), a);
+                        SubstDistributesOverApp(Lambda(zf, Pb_alt), Q, a, Var(b));
+                        SubstPushesIntoSafeLambda(zf, Pb_alt, a, Var(b));
+                        EqualTermsAreAlphaEquilvalent(QA, QA);
+                        ApplicationEquivalence(caSubstitution(Lambda(zf, Pb_alt), a, Var(b)), Lambda(zf, PbA), QA, QA);
+                        AlphaEquivTransitive(Mca,
+                                             caSubstitution(Application(Lambda(zf, Pb_alt), Q), a, Var(b)),
+                                             Application(caSubstitution(Lambda(zf, Pb_alt), a, Var(b)), QA));
+                        AlphaEquivTransitive(Mca,
+                                             Application(caSubstitution(Lambda(zf, Pb_alt), a, Var(b)), QA),
+                                             LHSapp);
+
+                        SubstAlphaEquivalence(Pb', z, zf);
+                        SubstRespectsBinderAlpha(z, Pb', zf, Pb'_alt, Q'');
+                        AlphaEquivTransitive(M', caSubstitution(Pb', z, Q''), caSubstitution(Pb'_alt, zf, Q''));
+                        EqualTermsAreAlphaEquilvalent(Var(b), Var(b));
+                        CaSubstEquivalence(M', Var(b), caSubstitution(Pb'_alt, zf, Q''), Var(b), a);
+                        SubstitutionLemma(Pb'_alt, Q'', Var(b), zf, a);
+                        AlphaEquivTransitive(M'ca,
+                                             caSubstitution(caSubstitution(Pb'_alt, zf, Q''), a, Var(b)),
+                                             caSubstitution(P2, zf, N2));
+
+                        ParRedBetaIntro(zf, PbA, QA, P2, N2, M'ca);
+                        AlphaEquivSymmetric(Mca, LHSapp);
+                        EqualTermsAreAlphaEquilvalent(M'ca, M'ca);
+                        CaSubsitutionOfVarDoesNotChangeHeightFORVARIABLES(Pb_alt, a, Var(b));
+                        CaSubsitutionOfVarDoesNotChangeHeightFORVARIABLES(Q, a, Var(b));
+                        ParallelReductionAlphaInvariance(LHSapp, M'ca, Mca, M'ca);
+                    }
+                    case _ => { assert false; }
+                }
+            }
+        }
+    }
+}
+
+lemma {:vcs_split_on_every_assert} ParRedAlphaUnderBinder(x:Id, B:LambdaTerm, R:LambdaTerm, x2:Id, B2arg:LambdaTerm)
+    requires parallelReduction(B, R)
+    requires alphaEquivalence(Lambda(x, B), Lambda(x2, B2arg))
+    ensures exists RR :: parallelReduction(B2arg, RR) && alphaEquivalence(Lambda(x2, RR), Lambda(x, R))
+    decreases lHeight(B), 2
+{
+    if x == x2 {
+        StripSameBinder(x, B, B2arg);
+        EqualTermsAreAlphaEquilvalent(R, R);
+        ParallelReductionAlphaInvariance(B, R, B2arg, R);
+        EqualTermsAreAlphaEquilvalent(Lambda(x2, R), Lambda(x, R));
+        assert parallelReduction(B2arg, R) && alphaEquivalence(Lambda(x2, R), Lambda(x, R));
+    } else {
+        BinderRenameNotFree(x, B, x2, B2arg);
+        ParRedPreservesNonFree(B, R, x2);
+        AvoidVarInTerm(B, x2);
+        var Bc :| alphaEquivalence(B, Bc) && !(x2 in vars(Bc));
+        AvoidVarInTerm(R, x2);
+        var Rc :| alphaEquivalence(R, Rc) && !(x2 in vars(Rc));
+
+        AlphaSameHeight(B, Bc);
+        ParallelReductionAlphaInvariance(B, R, Bc, Rc);
+
+        AlphaEquivSymmetric(B, Bc);
+        AlphaCongruenceLambda(x, Bc, B);
+        AlphaEquivTransitive(Lambda(x, Bc), Lambda(x, B), Lambda(x2, B2arg));
+
+        ParRedRename(Bc, Rc, x, x2);
+        var BcS := caSubstitution(Bc, x, Var(x2));
+        var RR := caSubstitution(Rc, x, Var(x2));
+        assert parallelReduction(BcS, RR);
+
+        CaSubstIsNaiveWhenFresh(Bc, x, x2);
+        SubstAlphaEquivalence(Bc, x, x2);
+        AlphaEquivSymmetric(Lambda(x, Bc), Lambda(x2, B2arg));
+        AlphaEquivTransitive(Lambda(x2, B2arg), Lambda(x, Bc), Lambda(x2, BcS));
+        StripSameBinder(x2, B2arg, BcS);
+        AlphaEquivSymmetric(B2arg, BcS);
+
+        CaSubsitutionOfVarDoesNotChangeHeightFORVARIABLES(Bc, x, Var(x2));
+        EqualTermsAreAlphaEquilvalent(RR, RR);
+        ParallelReductionAlphaInvariance(BcS, RR, B2arg, RR);
+
+        CaSubstIsNaiveWhenFresh(Rc, x, x2);
+        SubstAlphaEquivalence(Rc, x, x2);
+        AlphaEquivSymmetric(R, Rc);
+        AlphaCongruenceLambda(x, Rc, R);
+        AlphaEquivSymmetric(Lambda(x, Rc), Lambda(x2, RR));
+        AlphaEquivTransitive(Lambda(x2, RR), Lambda(x, Rc), Lambda(x, R));
+
+        assert parallelReduction(B2arg, RR) && alphaEquivalence(Lambda(x2, RR), Lambda(x, R));
+    }
+}
+
+
+
