LambdaCalculus/HelpingTheHelpers.dfy
@@ -1,0 +1,616 @@
+// include "ParallelReduction.dfy"
+// include "SubstitutionsAndSets.dfy"
+// include "LemmaA3.dfy"
+
+// lemma StripOuterBinder(t1:LambdaTerm, t2:LambdaTerm, w:Id, id1:seq<Id>, id2:seq<Id>)
+//     requires alphaEquivalence'(t1, t2, [w]+id1, [w]+id2)
+//     ensures alphaEquivalence'(t1, t2, id1, id2)
+//     decreases minim(lHeight(t1), lHeight(t2))
+//                 {
+//     match t1 {
+//         case Var(x) => {
+//             var z :| t2 == Var(z);
+//             findId_prepend(id1, x, w);
+//             findId_prepend(id2, z, w);
+//         }
+//         case Lambda(x, t1b) => {
+//             var z, t2b :| t2 == Lambda(z, t2b);
+//             assert ([w]+id1)+[x] == [w]+(id1+[x]);
+//             assert ([w]+id2)+[z] == [w]+(id2+[z]);
+//             StripOuterBinder(t1b, t2b, w, id1+[x], id2+[z]);
+//         }
+//         case Application(t1a, t1b) => {
+//             var t2a, t2b :| t2 == Application(t2a, t2b);
+//             StripOuterBinder(t1a, t2a, w, id1, id2);
+//             StripOuterBinder(t1b, t2b, w, id1, id2);
+//         }
+//     }
+// }
+
+// lemma StripSameBinder(w:Id, a:LambdaTerm, b:LambdaTerm)
+//     requires alphaEquivalence(Lambda(w,a), Lambda(w,b))
+//     ensures alphaEquivalence(a, b)
+// {
+//     assert []+[w] == [w];
+//     assert [w] == [w]+[];
+//     StripOuterBinder(a, b, w, [], []);
+// }
+
+// lemma FreeSubsetVars(t:LambdaTerm)
+//     ensures forall i:Id :: i in free(t) ==> i in vars(t)
+// {
+//     match t {
+//         case Var(_) => { }
+//         case Lambda(y,b) => { FreeSubsetVars(b); varsOfALambdaIncludesVarsofASubLambda(t); }
+//         case Application(a,b) => { FreeSubsetVars(a); FreeSubsetVars(b); varsOfALambdaIncludesVarsofASubLambda(t); }
+//     }
+// }
+
+// lemma CaSubstPrimeIsNaiveWhenFresh(M:LambdaTerm, x:Id, w:Id, ids:seq<Id>)
+//     requires allUnique(ids)
+//     requires includes(ids, vars(M))
+//     requires w in ids
+//     requires x in ids
+//     requires !(w in vars(M))
+//     ensures caSubstitution'(M, x, Var(w), ids) == substitution(M, x, Var(w))
+//     decreases lHeight(M)
+// {
+//     match M {
+//         case Var(y) => { }
+//         case Application(a, b) => {
+//             varsOfALambdaIncludesVarsofASubLambda(M);
+//             CaSubstPrimeIsNaiveWhenFresh(a, x, w, ids);
+//             CaSubstPrimeIsNaiveWhenFresh(b, x, w, ids);
+//         }
+//         case Lambda(z, P) => {
+//             if z == x {
+//             } else {
+//                 varsOfALambdaIncludesVarsofASubLambda(M);
+//                 assert z in vars(M);
+//                 assert w != z;
+//                 assert !(z in free(Var(w)));
+//                 assert !(w in vars(P));
+//                 CaSubstPrimeIsNaiveWhenFresh(P, x, w, ids);
+//             }
+//         }
+//     }
+// }
+
+// lemma CaSubstIsNaiveWhenFresh(M:LambdaTerm, x:Id, w:Id)
+//     requires !(w in vars(M))
+//     ensures caSubstitution(M, x, Var(w)) == substitution(M, x, Var(w))
+// {
+//     var ids := reunion(vars(M), vars(Var(w)));
+//     reunionIncludesBothSets(vars(M), vars(Var(w)));
+//     var safe_ids := addition(x, ids);
+//     CaSubstPrimeIsNaiveWhenFresh(M, x, w, safe_ids);
+// }
+
+// // Commutation of two naive variable-renamings (all four names distinct).
+// lemma SubstSubstSwapVars(P:LambdaTerm, x:Id, w:Id, z:Id, zz:Id)
+//     requires x != w && x != z && x != zz && w != z && w != zz && z != zz
+//     ensures substitution(substitution(P,x,Var(w)), z, Var(zz))
+//          == substitution(substitution(P,z,Var(zz)), x, Var(w))
+//     decreases lHeight(P)
+// {
+//     match P {
+//         case Var(u) => { }
+//         case Application(a,b) => {
+//             SubstSubstSwapVars(a,x,w,z,zz);
+//             SubstSubstSwapVars(b,x,w,z,zz);
+//         }
+//         case Lambda(u,Q) => {
+//             if u == x {
+//             } else if u == z {
+//             } else {
+//                 SubstSubstSwapVars(Q,x,w,z,zz);
+//             }
+//         }
+//     }
+// }
+
+
+// lemma {:vcs_split_on_every_assert} RenameThenSubstCapture(z:Id, P:LambdaTerm, x:Id, w:Id, N:LambdaTerm)
+//     requires !(w in vars(P))
+//     requires x != w && z != w && z != x
+//     requires z in free(N)
+//     ensures alphaEquivalence(caSubstitution(substitution(Lambda(z,P),x,Var(w)), w, N),
+//                              caSubstitution(Lambda(z,P), x, N))
+//     decreases lHeight(Lambda(z,P)), 0
+// {
+//     var A := Lambda(z,P);
+//     var sP := substitution(P,x,Var(w));
+//     assert substitution(A,x,Var(w)) == Lambda(z, sP);
+
+//     var s2 := addition(x, addition(z, addition(w, reunion(vars(P), vars(N)))));
+//     reunionIncludesBothSets(vars(P), vars(N));
+//     var zz := addAnUniqueId(s2)[0];
+//     assert !(zz in s2);
+//     assert zz != x && zz != z && zz != w;
+//     assert !(zz in vars(P)) && !(zz in vars(N));
+//     FreeSubsetVars(N);
+//     assert !(zz in free(N));
+
+//     var idsP := addition(w, vars(P));
+//     assert includes(idsP, vars(P));
+//     newIdsDueToSubstitution(P, x, Var(w), idsP);
+//     assert includes(idsP, vars(sP));
+//     assert !(zz in idsP);
+//     assert !(zz in vars(sP));
+
+//     var Pzz := substitution(P, z, Var(zz));
+//     var sPzz := substitution(sP, z, Var(zz));
+
+//     SubstSubstSwapVars(P, x, w, z, zz);
+//     assert sPzz == substitution(Pzz, x, Var(w));
+
+//     SubstAlphaEquivalence(P, z, zz);
+//     SubstAlphaEquivalence(sP, z, zz);
+
+//     EqualTermsAreAlphaEquilvalent(N, N);
+//     CaSubstEquivalence(Lambda(z,P), N, Lambda(zz,Pzz), N, x);
+//     SubstPushesIntoSafeLambda(zz, Pzz, x, N);
+//     var R := caSubstitution(A, x, N);
+//     AlphaEquivTransitive(R, caSubstitution(Lambda(zz,Pzz),x,N), Lambda(zz, caSubstitution(Pzz,x,N)));
+
+//     CaSubstEquivalence(Lambda(z,sP), N, Lambda(zz,sPzz), N, w);
+//     SubstPushesIntoSafeLambda(zz, sPzz, w, N);
+//     var L := caSubstitution(Lambda(z,sP), w, N);
+//     AlphaEquivTransitive(L, caSubstitution(Lambda(zz,sPzz),w,N), Lambda(zz, caSubstitution(sPzz,w,N)));
+
+//     var idsW := addition(zz, vars(P));
+//     assert includes(idsW, vars(P));
+//     newIdsDueToSubstitution(P, z, Var(zz), idsW);
+//     assert includes(idsW, vars(Pzz));
+//     assert !(w in idsW);
+//     assert !(w in vars(Pzz));
+
+//     subsitutionOfVarDoesNotChangeHeightFORVARIABLES(P, z, Var(zz));
+//     RenameThenSubst(Pzz, x, w, N);
+//     assert caSubstitution(sPzz,w,N) == caSubstitution(substitution(Pzz,x,Var(w)),w,N);
+//     AlphaCongruenceLambda(zz, caSubstitution(sPzz,w,N), caSubstitution(Pzz,x,N));
+
+//     AlphaEquivTransitive(L, Lambda(zz, caSubstitution(sPzz,w,N)), Lambda(zz, caSubstitution(Pzz,x,N)));
+//     AlphaEquivSymmetric(R, Lambda(zz, caSubstitution(Pzz,x,N)));
+//     AlphaEquivTransitive(L, Lambda(zz, caSubstitution(Pzz,x,N)), R);
+// }
+
+// lemma {:vcs_split_on_every_assert} RenameThenSubst(A:LambdaTerm, x:Id, w:Id, N:LambdaTerm)
+//     requires !(w in vars(A))
+//     requires x != w
+//     ensures alphaEquivalence(caSubstitution(substitution(A,x,Var(w)), w, N),
+//                              caSubstitution(A,x,N))
+//     decreases lHeight(A), 1
+// {
+//     match A {
+//         case Var(y) => {
+//             if y == x {
+//                 getVarCaSubstitution(Var(w), w, N);
+//                 getVarCaSubstitution(Var(x), x, N);
+//                 EqualTermsAreAlphaEquilvalent(caSubstitution(substitution(A,x,Var(w)),w,N), caSubstitution(A,x,N));
+//             } else {
+//                 assert y != w;
+//                 getVarCaSubstitution(Var(y), w, N);
+//                 getVarCaSubstitution(Var(y), x, N);
+//                 EqualTermsAreAlphaEquilvalent(caSubstitution(substitution(A,x,Var(w)),w,N), caSubstitution(A,x,N));
+//             }
+//         }
+//         case Application(a,b) => {
+//             varsOfALambdaIncludesVarsofASubLambda(A);
+//             assert !(w in vars(a)) && !(w in vars(b));
+//             var sa := substitution(a,x,Var(w));
+//             var sb := substitution(b,x,Var(w));
+//             assert substitution(A,x,Var(w)) == Application(sa, sb);
+
+//             SubstDistributesOverApp(sa, sb, w, N);
+//             SubstDistributesOverApp(a, b, x, N);
+
+//             RenameThenSubst(a,x,w,N);
+//             RenameThenSubst(b,x,w,N);
+
+//             ApplicationEquivalence(caSubstitution(sa,w,N), caSubstitution(a,x,N),
+//                                    caSubstitution(sb,w,N), caSubstitution(b,x,N));
+//             var L := caSubstitution(substitution(A,x,Var(w)),w,N);
+//             var R := caSubstitution(A,x,N);
+//             AlphaEquivSymmetric(R, Application(caSubstitution(a,x,N), caSubstitution(b,x,N)));
+//             AlphaEquivTransitive(L, Application(caSubstitution(sa,w,N), caSubstitution(sb,w,N)),
+//                                     Application(caSubstitution(a,x,N), caSubstitution(b,x,N)));
+//             AlphaEquivTransitive(L, Application(caSubstitution(a,x,N), caSubstitution(b,x,N)), R);
+//         }
+//         case Lambda(z,P) => {
+//             varsOfALambdaIncludesVarsofASubLambda(A);
+//             assert z in vars(A) && z != w;
+//             assert !(w in vars(P));
+//             if z == x {
+//                 assert substitution(A,x,Var(w)) == A;
+//                 FreeSubsetVars(A);
+//                 assert !(w in free(A));
+//                 NoFreeVariablesToReplace(A, w, N);
+//                 LambdaNullifiesSubstitution(P, x, N);
+//                 AlphaEquivSymmetric(caSubstitution(A,w,N), A);
+//                 EqualTermsAreAlphaEquilvalent(A, caSubstitution(A,x,N));
+//                 AlphaEquivTransitive(caSubstitution(A,w,N), A, caSubstitution(A,x,N));
+//             } else {
+//                 var sP := substitution(P,x,Var(w));
+//                 assert substitution(A,x,Var(w)) == Lambda(z, sP);
+//                 if !(z in free(N)) {
+//                     SubstPushesIntoSafeLambda(z, sP, w, N);
+//                     SubstPushesIntoSafeLambda(z, P, x, N);
+//                     RenameThenSubst(P,x,w,N);
+//                     AlphaCongruenceLambda(z, caSubstitution(sP,w,N), caSubstitution(P,x,N));
+
+//                     var L := caSubstitution(Lambda(z,sP), w, N);
+//                     var R := caSubstitution(A, x, N);
+//                     AlphaEquivTransitive(L, Lambda(z, caSubstitution(sP,w,N)), Lambda(z, caSubstitution(P,x,N)));
+//                     AlphaEquivSymmetric(R, Lambda(z, caSubstitution(P,x,N)));
+//                     AlphaEquivTransitive(L, Lambda(z, caSubstitution(P,x,N)), R);
+//                 } else {
+//                     RenameThenSubstCapture(z, P, x, w, N);
+//                 }
+//             }
+//         }
+//     }
+// }
+
+
+// lemma SubstRespectsBinderAlpha(x:Id, A:LambdaTerm, xx:Id, B:LambdaTerm, N:LambdaTerm)
+//     requires alphaEquivalence(Lambda(x,A), Lambda(xx,B))
+//     ensures alphaEquivalence(caSubstitution(A,x,N), caSubstitution(B,xx,N))
+// {
+//     reunionIncludesBothSets(vars(B), vars(N));
+//     var inner := reunion(vars(B), vars(N));
+//     var s := addition(x, addition(xx, reunion(vars(A), inner)));
+//     var w := addAnUniqueId(s)[0];
+//     assert !(w in s);
+//     assert w != x && w != xx;
+//     reunionIncludesBothSets(vars(A), inner);
+//     assert !(w in vars(A)) && !(w in vars(B)) && !(w in vars(N));
+
+//     var Aw := substitution(A, x, Var(w));
+//     var Bw := substitution(B, xx, Var(w));
+
+//     SubstAlphaEquivalence(A, x, w);
+//     SubstAlphaEquivalence(B, xx, w);
+//     AlphaEquivSymmetric(Lambda(x,A), Lambda(w,Aw));
+//     AlphaEquivTransitive(Lambda(w,Aw), Lambda(x,A), Lambda(xx,B));
+//     AlphaEquivTransitive(Lambda(w,Aw), Lambda(xx,B), Lambda(w,Bw));
+//     StripSameBinder(w, Aw, Bw);
+
+//                     EqualTermsAreAlphaEquilvalent(N, N);
+//     CaSubstEquivalence(Aw, N, Bw, N, w);
+
+//     RenameThenSubst(A, x, w, N);
+//     RenameThenSubst(B, xx, w, N);
+
+//     AlphaEquivSymmetric(caSubstitution(Aw,w,N), caSubstitution(A,x,N));
+//     AlphaEquivTransitive(caSubstitution(A,x,N), caSubstitution(Aw,w,N), caSubstitution(Bw,w,N));
+//     AlphaEquivTransitive(caSubstitution(A,x,N), caSubstitution(Bw,w,N), caSubstitution(B,xx,N));
+//                 }
+
+
+// // ===========================================================================
+// // Mutually-recursive layer for alpha-invariance of parallel reduction.
+// // ===========================================================================
+
+
+
+
+
+// lemma ParRedPreservesNonFree(M:LambdaTerm, M':LambdaTerm, y:Id)
+//     requires parallelReduction(M, M')
+//     requires !(y in free(M))
+//     ensures !(y in free(M'))
+//     decreases lHeight(M)
+// {
+//     if alphaEquivalence(M, M') {
+//         if y in free(M') { AlphaEquivSymmetric(M, M'); sameFreeForEquivalent(M', M, y); }
+//     } else {
+//         match M {
+//             case Var(_) => { }
+//             case Lambda(x, body) => {
+//                 var r :| parallelReduction(body, r) && alphaEquivalence(Lambda(x, r), M');
+//                 if y != x { ParRedPreservesNonFree(body, r, y); }
+//                 assert !(y in free(Lambda(x, r)));
+//                 if y in free(M') {
+//                     AlphaEquivSymmetric(Lambda(x, r), M');
+//                     sameFreeForEquivalent(M', Lambda(x, r), y);
+//                 }
+//             }
+//             case Application(P, Q) => {
+//                 if M'.Application? && parallelReduction(P, M'.t1) && parallelReduction(Q, M'.t2) {
+//                     ParRedPreservesNonFree(P, M'.t1, y);
+//                     ParRedPreservesNonFree(Q, M'.t2, y);
+//                 } else {
+//                     match P {
+//                         case Lambda(z, Pb) => {
+//                             var Pb', Q' :| parallelReduction(Pb, Pb') && parallelReduction(Q, Q')
+//                                            && alphaEquivalence(M', caSubstitution(Pb', z, Q'));
+//                             assert !(y in free(Q));
+//                             ParRedPreservesNonFree(Q, Q', y);
+//                             if y == z {
+//                                 SubstedVarNotFree(Pb', z, Q');
+//                             } else {
+//                                 assert !(y in free(Pb));
+//                                 ParRedPreservesNonFree(Pb, Pb', y);
+//                                 TheFreeOfCaSub(Pb', z, Q', y);
+//                             }
+//                             assert !(y in free(caSubstitution(Pb', z, Q')));
+//                             if y in free(M') {
+//                                 sameFreeForEquivalent(M', caSubstitution(Pb', z, Q'), y);
+//                             }
+//                         }
+//                         case _ => { assert false; }
+//                     }
+//                 }
+//             }
+//         }
+//     }
+// }
+
+// lemma AvoidVarInTerm(M:LambdaTerm, v:Id)
+//     requires !(v in free(M))
+//     ensures exists M' :: alphaEquivalence(M, M') && !(v in vars(M'))
+//     decreases lHeight(M)
+// {
+//     match M {
+//         case Var(y) => { EqualTermsAreAlphaEquilvalent(M, M); }
+//         case Application(P, Q) => {
+//             AvoidVarInTerm(P, v);
+//             var P' :| alphaEquivalence(P, P') && !(v in vars(P'));
+//             AvoidVarInTerm(Q, v);
+//             var Q' :| alphaEquivalence(Q, Q') && !(v in vars(Q'));
+//             ApplicationEquivalence(P, P', Q, Q');
+//             reunionIncludesBothSets(vars(P'), vars(Q'));
+//             assert !(v in vars(Application(P', Q')));
+//         }
+//         case Lambda(z, body) => {
+//             varsOfALambdaIncludesVarsofASubLambda(M);
+//             if z == v {
+//                 var zf := addAnUniqueId(vars(M))[0];
+//                 assert !(zf in vars(M)) && !(zf in vars(body));
+//                 var br := substitution(body, v, Var(zf));
+//                 SubstAlphaEquivalence(body, v, zf);
+//                 subsitutionOfVarDoesNotChangeHeightFORVARIABLES(body, v, Var(zf));
+//                 NaiveSubstRemovesVar(body, v, zf);
+//                 AvoidVarInTerm(br, v);
+//                 var br2 :| alphaEquivalence(br, br2) && !(v in vars(br2));
+//                 AlphaCongruenceLambda(zf, br, br2);
+//                 AlphaEquivTransitive(M, Lambda(zf, br), Lambda(zf, br2));
+//                 assert !(v in vars(Lambda(zf, br2)));
+//             } else {
+//                 assert !(v in free(body));
+//                 AvoidVarInTerm(body, v);
+//                 var body2 :| alphaEquivalence(body, body2) && !(v in vars(body2));
+//                 AlphaCongruenceLambda(z, body, body2);
+//                 assert !(v in vars(Lambda(z, body2)));
+//             }
+//         }
+//     }
+// }
+
+// lemma ParRedLambdaIntro(zf:Id, body:LambdaTerm, rr:LambdaTerm, t2:LambdaTerm)
+//     requires parallelReduction(body, rr) && alphaEquivalence(Lambda(zf, rr), t2)
+//     ensures parallelReduction(Lambda(zf, body), t2)
+// { }
+// lemma ParRedBetaIntro(zf:Id, PbA:LambdaTerm, QA:LambdaTerm, P2:LambdaTerm, N2:LambdaTerm, t2:LambdaTerm)
+//     requires parallelReduction(PbA, P2) && parallelReduction(QA, N2)
+//     requires alphaEquivalence(t2, caSubstitution(P2, zf, N2))
+//     ensures parallelReduction(Application(Lambda(zf, PbA), QA), t2)
+// { }
+// lemma ParRedCongIntro(PA:LambdaTerm, QA:LambdaTerm, PpA:LambdaTerm, QpA:LambdaTerm)
+//     requires parallelReduction(PA, PpA) && parallelReduction(QA, QpA)
+//     ensures parallelReduction(Application(PA, QA), Application(PpA, QpA))
+// { }
+
+// lemma {:vcs_split_on_every_assert} ParRedRename(M:LambdaTerm, M':LambdaTerm, a:Id, b:Id)
+//     requires parallelReduction(M, M')
+//     ensures parallelReduction(caSubstitution(M, a, Var(b)), caSubstitution(M', a, Var(b)))
+//     decreases lHeight(M), 1
+// {
+//     var Mca := caSubstitution(M, a, Var(b));
+//     var M'ca := caSubstitution(M', a, Var(b));
+//     if alphaEquivalence(M, M') {
+//         EqualTermsAreAlphaEquilvalent(Var(b), Var(b));
+//         CaSubstEquivalence(M, Var(b), M', Var(b), a);
+//         return;
+//     }
+//     match M {
+//         case Var(z) => { assert false; }
+//         case Lambda(z, body) => {
+//             var s :| parallelReduction(body, s) && alphaEquivalence(Lambda(z, s), M');
+//             var S := addition(a, addition(b, reunion(vars(M), reunion(vars(M'), vars(s)))));
+//             reunionIncludesBothSets(vars(M'), vars(s));
+//             reunionIncludesBothSets(vars(M), reunion(vars(M'), vars(s)));
+//             var zf := addAnUniqueId(S)[0];
+//             assert !(zf in S);
+//             assert zf != a && zf != b;
+//             varsOfALambdaIncludesVarsofASubLambda(M);
+//             assert !(zf in vars(M)) && !(zf in vars(M')) && !(zf in vars(s));
+//             assert !(zf in vars(body));
+
+//             var body_alt := substitution(body, z, Var(zf));
+//             var s_alt := substitution(s, z, Var(zf));
+
+//             ParRedRename(body, s, z, zf);
+//             CaSubstIsNaiveWhenFresh(body, z, zf);
+//             CaSubstIsNaiveWhenFresh(s, z, zf);
+//             assert parallelReduction(body_alt, s_alt);
+
+//             subsitutionOfVarDoesNotChangeHeightFORVARIABLES(body, z, Var(zf));
+//             ParRedRename(body_alt, s_alt, a, b);
+//             var PbA := caSubstitution(body_alt, a, Var(b));
+//             var rr := caSubstitution(s_alt, a, Var(b));
+//             assert parallelReduction(PbA, rr);
+
+//             SubstAlphaEquivalence(body, z, zf);
+//             EqualTermsAreAlphaEquilvalent(Var(b), Var(b));
+//             CaSubstEquivalence(M, Var(b), Lambda(zf, body_alt), Var(b), a);
+//             SubstPushesIntoSafeLambda(zf, body_alt, a, Var(b));
+//             AlphaEquivTransitive(Mca, caSubstitution(Lambda(zf, body_alt), a, Var(b)), Lambda(zf, PbA));
+
+//             SubstAlphaEquivalence(s, z, zf);
+//             AlphaEquivTransitive(Lambda(zf, s_alt), Lambda(z, s), M');
+//             CaSubstEquivalence(Lambda(zf, s_alt), Var(b), M', Var(b), a);
+//             SubstPushesIntoSafeLambda(zf, s_alt, a, Var(b));
+//             AlphaEquivSymmetric(caSubstitution(Lambda(zf, s_alt), a, Var(b)), Lambda(zf, rr));
+//             AlphaEquivTransitive(Lambda(zf, rr), caSubstitution(Lambda(zf, s_alt), a, Var(b)), M'ca);
+
+//             ParRedLambdaIntro(zf, PbA, rr, M'ca);
+//             AlphaEquivSymmetric(Mca, Lambda(zf, PbA));
+//             EqualTermsAreAlphaEquilvalent(M'ca, M'ca);
+//             CaSubsitutionOfVarDoesNotChangeHeightFORVARIABLES(body_alt, a, Var(b));
+//             ParallelReductionAlphaInvariance(Lambda(zf, PbA), M'ca, Mca, M'ca);
+//         }
+//         case Application(P, Q) => {
+//             if M'.Application? && parallelReduction(P, M'.t1) && parallelReduction(Q, M'.t2) {
+//                 var Pp := M'.t1;
+//                 var Qp := M'.t2;
+//                 SubstDistributesOverApp(P, Q, a, Var(b));
+//                 SubstDistributesOverApp(Pp, Qp, a, Var(b));
+//                 ParRedRename(P, Pp, a, b);
+//                 ParRedRename(Q, Qp, a, b);
+//                 var PA := caSubstitution(P, a, Var(b));
+//                 var QA := caSubstitution(Q, a, Var(b));
+//                 var PpA := caSubstitution(Pp, a, Var(b));
+//                 var QpA := caSubstitution(Qp, a, Var(b));
+//                 ParRedCongIntro(PA, QA, PpA, QpA);
+//                 AlphaEquivSymmetric(Mca, Application(PA, QA));
+//                 AlphaEquivSymmetric(M'ca, Application(PpA, QpA));
+//                 CaSubsitutionOfVarDoesNotChangeHeightFORVARIABLES(P, a, Var(b));
+//                 CaSubsitutionOfVarDoesNotChangeHeightFORVARIABLES(Q, a, Var(b));
+//                 ParallelReductionAlphaInvariance(Application(PA, QA), Application(PpA, QpA), Mca, M'ca);
+//             } else {
+//                 match P {
+//                     case Lambda(z, Pb) => {
+//                         var Pb', Q'' :| parallelReduction(Pb, Pb') && parallelReduction(Q, Q'')
+//                                         && alphaEquivalence(M', caSubstitution(Pb', z, Q''));
+//                         var S := addition(a, addition(b, reunion(vars(M), reunion(vars(M'),
+//                                     reunion(vars(Pb'), vars(Q''))))));
+//                         reunionIncludesBothSets(vars(Pb'), vars(Q''));
+//                         reunionIncludesBothSets(vars(M'), reunion(vars(Pb'), vars(Q'')));
+//                         reunionIncludesBothSets(vars(M), reunion(vars(M'), reunion(vars(Pb'), vars(Q''))));
+//                         var zf := addAnUniqueId(S)[0];
+//                         assert !(zf in S);
+//                         assert zf != a && zf != b;
+//                         varsOfALambdaIncludesVarsofASubLambda(M);
+//                         varsOfALambdaIncludesVarsofASubLambda(P);
+//                         assert !(zf in vars(M)) && !(zf in vars(M')) && !(zf in vars(Pb')) && !(zf in vars(Q''));
+//                         assert !(zf in vars(P));
+//                         assert !(zf in vars(Pb)) && !(zf in vars(Q));
+
+//                         var Pb_alt := substitution(Pb, z, Var(zf));
+//                         var Pb'_alt := substitution(Pb', z, Var(zf));
+
+//                         assert parallelReduction(Pb, Pb');
+//                         assert lHeight(Pb) < lHeight(M);
+//                         ParRedRename(Pb, Pb', z, zf);
+//                         CaSubstIsNaiveWhenFresh(Pb, z, zf);
+//                         CaSubstIsNaiveWhenFresh(Pb', z, zf);
+//                         assert parallelReduction(Pb_alt, Pb'_alt);
+
+//                         subsitutionOfVarDoesNotChangeHeightFORVARIABLES(Pb, z, Var(zf));
+//                         var PbA := caSubstitution(Pb_alt, a, Var(b));
+//                         var QA := caSubstitution(Q, a, Var(b));
+//                         var P2 := caSubstitution(Pb'_alt, a, Var(b));
+//                         var N2 := caSubstitution(Q'', a, Var(b));
+
+//                         ParRedRename(Pb_alt, Pb'_alt, a, b);
+//                         ParRedRename(Q, Q'', a, b);
+//                         assert parallelReduction(PbA, P2);
+//                         assert parallelReduction(QA, N2);
+
+//                         var LHSapp := Application(Lambda(zf, PbA), QA);
+
+//                         SubstAlphaEquivalence(Pb, z, zf);
+//                         EqualTermsAreAlphaEquilvalent(Q, Q);
+//                         ApplicationEquivalence(Lambda(z, Pb), Lambda(zf, Pb_alt), Q, Q);
+//                         EqualTermsAreAlphaEquilvalent(Var(b), Var(b));
+//                         CaSubstEquivalence(M, Var(b), Application(Lambda(zf, Pb_alt), Q), Var(b), a);
+//                         SubstDistributesOverApp(Lambda(zf, Pb_alt), Q, a, Var(b));
+//                         SubstPushesIntoSafeLambda(zf, Pb_alt, a, Var(b));
+//                         EqualTermsAreAlphaEquilvalent(QA, QA);
+//                         ApplicationEquivalence(caSubstitution(Lambda(zf, Pb_alt), a, Var(b)), Lambda(zf, PbA), QA, QA);
+//                         AlphaEquivTransitive(Mca,
+//                                              caSubstitution(Application(Lambda(zf, Pb_alt), Q), a, Var(b)),
+//                                              Application(caSubstitution(Lambda(zf, Pb_alt), a, Var(b)), QA));
+//                         AlphaEquivTransitive(Mca,
+//                                              Application(caSubstitution(Lambda(zf, Pb_alt), a, Var(b)), QA),
+//                                              LHSapp);
+
+//                         SubstAlphaEquivalence(Pb', z, zf);
+//                         SubstRespectsBinderAlpha(z, Pb', zf, Pb'_alt, Q'');
+//                         AlphaEquivTransitive(M', caSubstitution(Pb', z, Q''), caSubstitution(Pb'_alt, zf, Q''));
+//                         EqualTermsAreAlphaEquilvalent(Var(b), Var(b));
+//                         CaSubstEquivalence(M', Var(b), caSubstitution(Pb'_alt, zf, Q''), Var(b), a);
+//                         SubstitutionLemma(Pb'_alt, Q'', Var(b), zf, a);
+//                         AlphaEquivTransitive(M'ca,
+//                                              caSubstitution(caSubstitution(Pb'_alt, zf, Q''), a, Var(b)),
+//                                              caSubstitution(P2, zf, N2));
+
+//                         ParRedBetaIntro(zf, PbA, QA, P2, N2, M'ca);
+//                         AlphaEquivSymmetric(Mca, LHSapp);
+//                         EqualTermsAreAlphaEquilvalent(M'ca, M'ca);
+//                         CaSubsitutionOfVarDoesNotChangeHeightFORVARIABLES(Pb_alt, a, Var(b));
+//                         CaSubsitutionOfVarDoesNotChangeHeightFORVARIABLES(Q, a, Var(b));
+//                         ParallelReductionAlphaInvariance(LHSapp, M'ca, Mca, M'ca);
+//                     }
+//                     case _ => { assert false; }
+//                 }
+//             }
+//         }
+//     }
+// }
+
+// lemma {:vcs_split_on_every_assert} ParRedAlphaUnderBinder(x:Id, B:LambdaTerm, R:LambdaTerm, x2:Id, B2arg:LambdaTerm)
+//     requires parallelReduction(B, R)
+//     requires alphaEquivalence(Lambda(x, B), Lambda(x2, B2arg))
+//     ensures exists RR :: parallelReduction(B2arg, RR) && alphaEquivalence(Lambda(x2, RR), Lambda(x, R))
+//     decreases lHeight(B), 2
+// {
+//     if x == x2 {
+//         StripSameBinder(x, B, B2arg);
+//         EqualTermsAreAlphaEquilvalent(R, R);
+//         ParallelReductionAlphaInvariance(B, R, B2arg, R);
+//         EqualTermsAreAlphaEquilvalent(Lambda(x2, R), Lambda(x, R));
+//         assert parallelReduction(B2arg, R) && alphaEquivalence(Lambda(x2, R), Lambda(x, R));
+//     } else {
+//         BinderRenameNotFree(x, B, x2, B2arg);
+//         ParRedPreservesNonFree(B, R, x2);
+//         AvoidVarInTerm(B, x2);
+//         var Bc :| alphaEquivalence(B, Bc) && !(x2 in vars(Bc));
+//         AvoidVarInTerm(R, x2);
+//         var Rc :| alphaEquivalence(R, Rc) && !(x2 in vars(Rc));
+
+//         AlphaSameHeight(B, Bc);
+//         ParallelReductionAlphaInvariance(B, R, Bc, Rc);
+
+//         AlphaEquivSymmetric(B, Bc);
+//         AlphaCongruenceLambda(x, Bc, B);
+//         AlphaEquivTransitive(Lambda(x, Bc), Lambda(x, B), Lambda(x2, B2arg));
+
+//         ParRedRename(Bc, Rc, x, x2);
+//         var BcS := caSubstitution(Bc, x, Var(x2));
+//         var RR := caSubstitution(Rc, x, Var(x2));
+//         assert parallelReduction(BcS, RR);
+
+//         CaSubstIsNaiveWhenFresh(Bc, x, x2);
+//         SubstAlphaEquivalence(Bc, x, x2);
+//         AlphaEquivSymmetric(Lambda(x, Bc), Lambda(x2, B2arg));
+//         AlphaEquivTransitive(Lambda(x2, B2arg), Lambda(x, Bc), Lambda(x2, BcS));
+//         StripSameBinder(x2, B2arg, BcS);
+//         AlphaEquivSymmetric(B2arg, BcS);
+
+//         CaSubsitutionOfVarDoesNotChangeHeightFORVARIABLES(Bc, x, Var(x2));
+//         EqualTermsAreAlphaEquilvalent(RR, RR);
+//         ParallelReductionAlphaInvariance(BcS, RR, B2arg, RR);
+
+//         CaSubstIsNaiveWhenFresh(Rc, x, x2);
+//         SubstAlphaEquivalence(Rc, x, x2);
+//         AlphaEquivSymmetric(R, Rc);
+//         AlphaCongruenceLambda(x, Rc, R);
+//         AlphaEquivSymmetric(Lambda(x, Rc), Lambda(x2, RR));
+//         AlphaEquivTransitive(Lambda(x2, RR), Lambda(x, Rc), Lambda(x, R));
+
+//         assert parallelReduction(B2arg, RR) && alphaEquivalence(Lambda(x2, RR), Lambda(x, R));
+//     }
+// }
