LambdaCalculus/LemmaA2.dfy
@@ -1,0 +1,231 @@
+include "HelperLemmasForA2.dfy"
+
+lemma SubstitutionLemma (M:LambdaTerm,N:LambdaTerm,P:LambdaTerm,x:Id,y:Id)
+    requires x!=y
+    requires !(x in free(P))
+    ensures alphaEquivalence(caSubstitution(caSubstitution(M,x,N),y,P),caSubstitution(caSubstitution(M,y,P),x,caSubstitution(N,y,P)))
+    decreases lHeight(M)
+
+{
+    match M
+        case Application(M1,M2) =>
+        {
+            SubstitutionLemma(M1, N, P, x, y);
+            SubstitutionLemma(M2, N, P, x, y);
+
+            var N_sub_y := caSubstitution(N, y, P);
+
+            var M1_left := caSubstitution(caSubstitution(M1, x, N), y, P);
+            var M1_right := caSubstitution(caSubstitution(M1, y, P), x, N_sub_y);
+            var M2_left := caSubstitution(caSubstitution(M2, x, N), y, P);
+            var M2_right := caSubstitution(caSubstitution(M2, y, P), x, N_sub_y);
+
+            var app_left := Application(M1_left, M2_left);
+            var app_right := Application(M1_right, M2_right);
+            
+            ApplicationEquivalence(M1_left, M1_right, M2_left, M2_right);
+
+            var M_left_actual := caSubstitution(caSubstitution(M, x, N), y, P);
+            var M_right_actual := caSubstitution(caSubstitution(M, y, P), x, N_sub_y);
+
+            var inner_left := caSubstitution(M, x, N);
+            var inner_left_dist := Application(caSubstitution(M1, x, N), caSubstitution(M2, x, N));
+            
+            SubstDistributesOverApp(M1, M2, x, N);
+             EqualTermsAreAlphaEquilvalent(P, P);
+             assert alphaEquivalence(inner_left,inner_left_dist);
+             assert alphaEquivalence(P,P);
+             CaSubstEquivalence(inner_left,P, inner_left_dist, P, y);
+            
+            var mid_left := caSubstitution(inner_left_dist, y, P);
+            SubstDistributesOverApp(caSubstitution(M1, x, N), caSubstitution(M2, x, N), y, P);
+           AlphaEquivTransitive(M_left_actual, mid_left, app_left);
+
+            var inner_right := caSubstitution(M, y, P);
+            var inner_right_dist := Application(caSubstitution(M1, y, P), caSubstitution(M2, y, P));
+            
+            SubstDistributesOverApp(M1, M2, y, P);
+            EqualTermsAreAlphaEquilvalent(N_sub_y, N_sub_y);
+            CaSubstEquivalence(inner_right,N_sub_y ,inner_right_dist, N_sub_y, x);
+            
+            var mid_right := caSubstitution(inner_right_dist, x, N_sub_y);
+            SubstDistributesOverApp(caSubstitution(M1, y, P), caSubstitution(M2, y, P), x, N_sub_y);
+            AlphaEquivTransitive(M_right_actual, mid_right, app_right);
+
+            AlphaEquivSymmetric(M_right_actual, app_right);
+            AlphaEquivTransitive(M_left_actual, app_left, app_right);
+            AlphaEquivTransitive(M_left_actual, app_right, M_right_actual);
+
+            assert alphaEquivalence(caSubstitution(caSubstitution(M,x,N),y,P),caSubstitution(caSubstitution(M,y,P),x,caSubstitution(N,y,P)));
+        }
+        case Lambda(z,M')=>
+        {
+                var P_and_M := reunion(freeVec(P), vars(M'));
+                var N_P_M := reunion(freeVec(N), P_and_M);
+                var safe_ids := addition(x, addition(y, N_P_M));
+
+                var new_id := addAnUniqueId(safe_ids)[0];
+
+                assert !(new_id in safe_ids);
+                assert new_id != x && new_id != y;
+
+                NotInReunionSoNotInBoth(freeVec(N), P_and_M, new_id);
+                assert !(new_id in freeVec(N));
+                assert !(new_id in free(N));
+
+                NotInReunionSoNotInBoth(freeVec(P), vars(M'), new_id);
+                assert !(new_id in freeVec(P));
+                assert !(new_id in free(P));
+                assert !(new_id in vars(M'));
+
+                var new_M := Lambda(new_id, substitution(M', z, Var(new_id)));
+
+                SubstAlphaEquivalence(M', z, new_id);
+
+                var safe_body := substitution(M', z, Var(new_id));
+                assert alphaEquivalence(Lambda(z, M'), Lambda(new_id, safe_body));
+
+                assert alphaEquivalence(M, new_M);
+
+                subsitutionOfVarDoesNotChangeHeightFORVARIABLES(M', z, Var(new_id));
+                assert lHeight(safe_body) == lHeight(M') < lHeight(M);
+                SubstitutionLemma(safe_body, N, P, x, y);
+
+                var M'_left  := caSubstitution(caSubstitution(safe_body, x, N), y, P);
+                var M'_right := caSubstitution(caSubstitution(safe_body, y, P), x, caSubstitution(N, y, P));
+                assert alphaEquivalence(M'_left, M'_right);
+
+                AlphaCongruenceLambda(new_id, M'_left, M'_right);
+                var left_result  := Lambda(new_id, M'_left);
+                var right_result := Lambda(new_id, M'_right);   
+                assert alphaEquivalence(left_result, right_result);
+
+
+
+                var inner_left_sub := caSubstitution(new_M, x, N);
+                assert x != new_id;
+
+                SubstPushesIntoSafeLambda(new_id, safe_body, x, N);
+                var pushed_inner_left := Lambda(new_id, caSubstitution(safe_body, x, N));
+
+
+                EqualTermsAreAlphaEquilvalent(P, P);
+                CaSubstEquivalence(inner_left_sub, P, pushed_inner_left, P, y);
+                var outer_left_sub := caSubstitution(inner_left_sub, y, P);
+
+
+                SubstPushesIntoSafeLambda(new_id, caSubstitution(safe_body, x, N), y, P);
+
+                AlphaEquivTransitive(outer_left_sub,
+                                    caSubstitution(pushed_inner_left, y, P),
+                                    left_result);
+
+                var N_sub_y := caSubstitution(N, y, P);
+                var actual_left := caSubstitution(caSubstitution(M, x, N), y, P);
+
+                EqualTermsAreAlphaEquilvalent(N, N);
+                CaSubstEquivalence(M, N, new_M, N, x);
+                CaSubstEquivalence(caSubstitution(M, x, N), P,
+                                caSubstitution(new_M, x, N), P, y);
+
+                AlphaEquivTransitive(actual_left, outer_left_sub, left_result);
+
+
+                var inner_right_sub := caSubstitution(new_M, y, P);
+                SubstPushesIntoSafeLambda(new_id, safe_body, y, P);
+                var pushed_inner_right := Lambda(new_id, caSubstitution(safe_body, y, P));
+
+
+                EqualTermsAreAlphaEquilvalent(N_sub_y, N_sub_y);
+                CaSubstEquivalence(inner_right_sub, N_sub_y,
+                                pushed_inner_right, N_sub_y, x);
+                var outer_right_sub := caSubstitution(inner_right_sub, x, N_sub_y);
+
+
+                TheFreeOfCaSub(N, y, P, new_id);
+
+                SubstPushesIntoSafeLambda(new_id, caSubstitution(safe_body, y, P), x, N_sub_y);
+
+                AlphaEquivTransitive(outer_right_sub,
+                                    caSubstitution(pushed_inner_right, x, N_sub_y),
+                                    right_result);
+
+
+                var actual_right := caSubstitution(caSubstitution(M, y, P), x, N_sub_y);
+
+                EqualTermsAreAlphaEquilvalent(P, P);
+                CaSubstEquivalence(M, P, new_M, P, y);
+                CaSubstEquivalence(caSubstitution(M, y, P), N_sub_y,
+                                caSubstitution(new_M, y, P), N_sub_y, x);
+
+
+                AlphaEquivTransitive(actual_left, left_result, right_result);
+                AlphaEquivSymmetric(outer_right_sub, right_result);
+                AlphaEquivTransitive(actual_left, right_result, outer_right_sub);
+                AlphaEquivSymmetric(actual_right, outer_right_sub);
+                AlphaEquivTransitive(actual_left, outer_right_sub, actual_right);
+
+            assert alphaEquivalence(
+                caSubstitution(caSubstitution(M, x, N), y, P),
+                caSubstitution(caSubstitution(M, y, P), x, caSubstitution(N, y, P))
+            );
+        }
+        case Var(z) => {
+            if (z == x) {
+                var partial_result_left := caSubstitution(M, x, N);
+                assert partial_result_left == N;
+                
+                var left_result := caSubstitution(N, y, P);
+
+                var partial_result_right := caSubstitution(M, y, P);
+                assert partial_result_right == M;
+                
+                var N_sub := caSubstitution(N, y, P);
+                var right_result := caSubstitution(partial_result_right, x, N_sub);
+                assert right_result == N_sub; 
+
+                assert left_result == right_result;
+                EqualTermsAreAlphaEquilvalent(left_result, right_result);
+            }
+            else if (z == y) {
+                var partial_result_left := caSubstitution(M, x, N);
+                assert partial_result_left == M; // Because x != y
+                
+                var left_result := caSubstitution(M, y, P);
+                assert left_result == P; 
+
+                var partial_result_right := caSubstitution(M, y, P);
+                assert partial_result_right == P; 
+                
+                var N_sub := caSubstitution(N, y, P);
+                
+                var right_result := caSubstitution(P, x, N_sub); 
+
+                NoFreeVariablesToReplace(P, x, N_sub);
+
+                AlphaEquivSymmetric(right_result, P);
+                assert alphaEquivalence(left_result, right_result);
+
+            }
+            else {
+                var partial_result_left := caSubstitution(M, x, N);
+                assert partial_result_left == M;
+                
+                var left_result := caSubstitution(partial_result_left, y, P);
+                assert left_result == M;
+
+                var partial_result_right := caSubstitution(M, y, P);
+                assert partial_result_right == M;
+                
+                var N_sub := caSubstitution(N, y, P);
+                var right_result := caSubstitution(partial_result_right, x, N_sub);
+                assert right_result == M;
+
+                assert left_result == right_result;
+                EqualTermsAreAlphaEquilvalent(left_result, right_result);
+            }
+        } 
+    
+    
+
+}
