LambdaCalculus/LemmaA5AndA6.dfy
@@ -1,0 +1,42 @@
+include "ParallelReduction.dfy"
+lemma LambdaParallelLemma (M:LambdaTerm,N:LambdaTerm,x:Id) // LEMMA A5
+    requires parallelReduction(Lambda(x,M),N)
+    ensures exists M': LambdaTerm :: parallelReduction(M, M') && alphaEquivalence(Lambda(x, M'), N)
+{
+    if alphaEquivalence(Lambda(x, M), N) {
+        ParallelReductionIsReflexive(M);
+    } 
+
+}
+
+
+lemma AlphaParallelLemma(M: LambdaTerm, N: LambdaTerm, L: LambdaTerm) // LEMMA A6
+
+    requires parallelReduction(Application(M, N), L)
+    ensures 
+        (exists M': LambdaTerm, N': LambdaTerm :: 
+            parallelReduction(M, M') && parallelReduction(N, N') && alphaEquivalence(Application(M', N'), L))
+        ||
+        (M.Lambda? && 
+         exists P': LambdaTerm, N': LambdaTerm :: 
+            parallelReduction(M.t, P') && parallelReduction(N, N') && alphaEquivalence(L, caSubstitution(P', M.x, N')))
+{
+
+    if alphaEquivalence(Application(M, N), L) {
+        ParallelReductionIsReflexive(M);
+        ParallelReductionIsReflexive(N);
+        assert parallelReduction(M, M);
+        assert parallelReduction(N, N);
+        assert alphaEquivalence(Application(M, N), L);
+    } 
+    else {
+            
+        if rule3(Application(M,N),L) {
+            match L 
+                case Application(M',N') =>{
+                    EqualTermsAreAlphaEquilvalent(Application(M', N'), L);
+                    assert parallelReduction(M, M') && parallelReduction(N, N') && alphaEquivalence(Application(M', N'), L);
+                }
+        } 
+    }
+}
