LambdaCalculus/ParallelReduction.dfy
@@ -1,0 +1,86 @@
+include "AlphaEquivalence.dfy"
+
+
+
+ghost predicate parallelReduction(t1:LambdaTerm, t2:LambdaTerm)
+    decreases lHeight(t1)
+{
+    alphaEquivalence(t1, t2) || //rule 1 
+    match t1
+        case Application(t1a, t1b) =>
+            (match t2
+                case Application(t2a, t2b) =>
+                    parallelReduction(t1a, t2a) && parallelReduction(t1b, t2b)
+                case _ => false)
+            ||
+            (match t1a
+                case Lambda(x, M) =>
+                    exists M': LambdaTerm, N': LambdaTerm ::
+                        (assert lHeight(M) < lHeight(t1); parallelReduction(M, M'))
+                        && parallelReduction(t1b, N')
+                        && alphaEquivalence(t2, caSubstitution(M', x, N'))   
+                case _ => false)
+        case Lambda(x, body1) =>
+            exists r: LambdaTerm ::
+                parallelReduction(body1, r) && alphaEquivalence(Lambda(x, r), t2)
+        case _ => false
+}
+
+ghost predicate rule2(t1:LambdaTerm,t2:LambdaTerm) 
+    ensures rule2(t1,t2) ==> parallelReduction(t1,t2)
+{
+    match t1 
+        case Lambda(x, body1) =>
+            exists r: LambdaTerm ::
+                parallelReduction(body1, r) && alphaEquivalence(Lambda(x, r), t2)
+        case _=> false
+}
+ghost predicate rule3(t1:LambdaTerm,t2:LambdaTerm)
+    ensures rule3(t1,t2) ==> parallelReduction(t1,t2)
+{
+    match t1
+        case Application(t1a, t1b) =>
+            (match t2
+                case Application(t2a, t2b) =>
+                    parallelReduction(t1a, t2a) && parallelReduction(t1b, t2b)
+                case _ => false)
+        case _ => false
+}
+ghost predicate rule4(t1:LambdaTerm,t2:LambdaTerm)
+    ensures rule4(t1,t2) ==> parallelReduction(t1,t2)
+{
+    match t1
+        case Application(t1a, t1b) =>(match t1a
+                                            case Lambda(x, M) =>
+                                                exists M': LambdaTerm, N': LambdaTerm ::
+                                                (assert lHeight(M) < lHeight(t1); parallelReduction(M, M'))
+                                                && parallelReduction(t1b, N')
+                                                && alphaEquivalence(t2, caSubstitution(M', x, N'))   
+                                    case _ => false)
+        case _=> false
+}
+
+
+lemma ParallelReductionIsReflexive (t:LambdaTerm)
+    ensures parallelReduction(t,t)
+{
+    EqualTermsAreAlphaEquilvalent(t,t);
+}
+
+
+lemma ParallelReductionIsBasedOnFourRules(t1:LambdaTerm,t2:LambdaTerm)
+    requires parallelReduction(t1,t2)
+    ensures alphaEquivalence(t1,t2) || rule2(t1,t2) || rule3(t1,t2) || rule4(t1,t2)
+{
+
+}
+
+
+lemma FourRulesDefineParallelReduction (t1:LambdaTerm,t2:LambdaTerm)
+    requires alphaEquivalence(t1,t2) || rule2(t1,t2) || rule3(t1,t2) || rule4(t1,t2)
+    ensures parallelReduction(t1,t2)
+{
+
+}
+
+
