LambdaCalculus/ParallelReductionClosure.dfy
@@ -1,0 +1,101 @@
+include "BetaReduction.dfy"
+include "LemmaA5AndA6.dfy"
+include "HelperLemmasForA3.dfy"
+include "Diamond.dfy"
+
+
+ghost predicate parallelReductionInNSteps(t1:LambdaTerm,t2:LambdaTerm,n:nat)
+    decreases n
+{
+    if n==0 then alphaEquivalence(t1,t2)
+    else 
+    exists t':LambdaTerm:: parallelReduction(t1,t') && parallelReductionInNSteps(t',t2,n-1)
+}
+
+ghost predicate parallelReductionClosure(t1:LambdaTerm,t2:LambdaTerm)
+{
+    exists n:nat::parallelReductionInNSteps(t1,t2,n)
+}
+
+lemma parallelReductionClosureReflexive(t1:LambdaTerm)
+    ensures parallelReductionClosure(t1,t1)
+{
+    EqualTermsAreAlphaEquilvalent(t1,t1);
+    assert alphaEquivalence(t1,t1);
+    assert parallelReductionInNSteps(t1,t1,0);
+}
+lemma ParClosurePrepend(a:LambdaTerm, b:LambdaTerm, c:LambdaTerm)   
+    requires parallelReduction(a, b)
+    requires parallelReductionClosure(b, c)
+    ensures parallelReductionClosure(a, c)
+{
+    var n:nat :| parallelReductionInNSteps(b, c, n);
+    assert parallelReductionInNSteps(a, c, n+1);     
+}
+lemma StripLemma(a:LambdaTerm,b:LambdaTerm,c:LambdaTerm,n:nat)
+    requires parallelReduction(a, b)
+    requires parallelReductionInNSteps(a, c, n)
+    ensures exists d:LambdaTerm ::parallelReductionClosure(b, d) && parallelReduction(c, d)
+    decreases n
+{
+    if n==0{
+
+        assert alphaEquivalence(a,c);
+        assert parallelReduction(a,b);
+        EqualTermsAreAlphaEquilvalent(b,b);
+        ParallelReductionAlphaInvariance(a,b,c,b);
+        assert parallelReduction(b,b);
+        assert parallelReduction(c,b);
+        assert parallelReductionInNSteps(b,b,0);
+        assert parallelReductionInNSteps(c,b,1);
+
+    }
+    else
+    {
+        var next_a :| parallelReduction(a, next_a) && parallelReductionInNSteps(next_a, c, n-1);
+        DiamondLemma(a, b, next_a);                    
+        var e :| parallelReduction(b, e) && parallelReduction(next_a, e);
+        StripLemma(next_a, e, c, n-1);                  
+        var d :| parallelReductionClosure(e, d) && parallelReduction(c, d);
+        ParClosurePrepend(b, e, d);                    
+        assert parallelReductionClosure(b, d) && parallelReduction(c, d);
+    }
+}
+
+lemma ClosureDiamond(a:LambdaTerm, b:LambdaTerm, c:LambdaTerm, n:nat)
+    requires parallelReductionInNSteps(a, b, n)
+    requires parallelReductionClosure(a, c)
+    ensures exists d:LambdaTerm :: parallelReductionClosure(b, d) && parallelReductionClosure(c, d)
+    decreases n
+{
+    if (n==0)
+    {
+        assert alphaEquivalence(a, b);
+        AlphaEquivSymmetric(a, b);                
+        ParClosurePrepend(b, a, c);                
+        parallelReductionClosureReflexive(c);     
+        assert parallelReductionClosure(b, c) && parallelReductionClosure(c, c);
+        
+    }
+    else
+    {
+        var a_next :| parallelReduction(a, a_next) && parallelReductionInNSteps(a_next, b, n-1);
+        var m:nat :| parallelReductionInNSteps(a, c, m);
+        StripLemma(a, a_next, c, m);                    
+        var e :| parallelReductionClosure(a_next, e) && parallelReduction(c, e);
+        ClosureDiamond(a_next, b, e, n-1);             
+        var d :| parallelReductionClosure(b, d) && parallelReductionClosure(e, d);
+        ParClosurePrepend(c, e, d);                
+        assert parallelReductionClosure(b, d) && parallelReductionClosure(c, d);
+    }
+}
+
+
+lemma ParallelClosureHasDiamond(a:LambdaTerm, b:LambdaTerm, c:LambdaTerm)
+    requires parallelReductionClosure(a, b)
+    requires parallelReductionClosure(a, c)
+    ensures exists d:LambdaTerm :: parallelReductionClosure(b, d) && parallelReductionClosure(c, d)
+{
+    var m:nat :| parallelReductionInNSteps(a, b, m);
+    ClosureDiamond(a, b, c, m);
+}
